code/ecdsap256/Hacl.Impl.P256.PointDouble.fsti
@@ -31,25 +31,24 @@ val point_double: #c: curve -> p: point c -> result: point c -> tempBuffer: lbuf
     eq_or_disjoint p result /\
     (
       let prime = getPrime c in 
-      let len = uint_v (getCoordinateLenU64 c) in
-      as_nat c h (gsub p (size 0) (size len)) < prime /\ 
-      as_nat c h (gsub p (size len) (size len)) < prime /\
-      as_nat c h (gsub p (size (2 * len)) (size len)) < prime
+      let len = getCoordinateLenU64 c in
+      as_nat c h (gsub p (size 0) len) < prime /\ 
+      as_nat c h (gsub p len len) < prime /\
+      as_nat c h (gsub p (size 2 *! len) len) < prime
     )
   )
   (ensures fun h0 _ h1 -> modifies (loc tempBuffer |+| loc result)  h0 h1 /\  
     (
       let prime = getPrime c in 
-      let len = uint_v (getCoordinateLenU64 c) in 
+      let len = getCoordinateLenU64 c in 
       
-      as_nat c h1 (gsub result (size 0) (size len)) < prime /\ 
-      as_nat c h1 (gsub result (size len) (size len)) < prime /\
-      as_nat c h1 (gsub result (size (2 * len)) (size len)) < prime /\ 
+      as_nat c h1 (gsub result (size 0) len) < prime /\ 
+      as_nat c h1 (gsub result len len) < prime /\
+      as_nat c h1 (gsub result (size 2 *! len) len) < prime /\ 
       
       (
-	let x, y, z = gsub p (size 0) (size len), gsub p (size len) (size len), gsub p (size (2 * len)) (size len) in 
-	let x3, y3, z3 = gsub result (size 0) (size len), gsub result (size len) (size len), gsub result (size (2 * len)) (size len) in 
-      
+	let x, y, z = gsub p (size 0) len, gsub p len len, gsub p (size 2 *! len) len in 
+	let x3, y3, z3 = gsub result (size 0) len, gsub result len len, gsub result (size 2 *! len) len in       
 	let xD, yD, zD = fromDomain_ #c (as_nat c h0 x), fromDomain_ #c (as_nat c h0 y), fromDomain_ #c (as_nat c h0 z) in 
 	let x3D, y3D, z3D = fromDomain_ #c (as_nat c h1 x3), fromDomain_ #c (as_nat c h1 y3), fromDomain_ #c (as_nat c h1 z3) in
 	let xN, yN, zN = _point_double #c (xD, yD, zD) in 
